examples/rel/ifc_reify.fst
@@ -10,34 +10,39 @@ type label =
 
 type env = id ->  Tot label
 
-type low_equiv (env:env) (h : rel heap)  = 
-  forall (x:id). (Low? (env x) ==> sel (R?.l h) x = sel (R?.r h) x)
+type low_equiv (env:env) (h : rel heap)  =
+  forall (x:id). {:pattern (Low? (env x))} (Low? (env x) ==> sel (R?.l h) x = sel (R?.r h) x)
 
-reifiable let p1 x y hi = 
-  if read hi = 0 then 
-    write x (read x + read y) 
-  else 
-    write x (read x + read y + read hi);
-  write x (read x - read hi)
+reifiable let p1 x y hi =
+  if read hi = 0 then
+    let vx = read x in
+    let vy = read y in
+    write x (vx + vy)
+  else
+    let vx = read x in
+    let vy = read y in
+    let vhi = read hi in
+    write x (vx + vy + vhi);
+  let vx = read x in
+  let vhi = read hi in
+  write x (vx - vhi)
 
 let p1_r x y hi h = (* normalize_term *) (snd (reify (p1 x y hi) h))
 
-val p1_x (x y hi : id) (h:heap) : 
-  Lemma 
-  (requires (x <> y /\ x <> hi /\ y <> hi))
-  (ensures  (fun h' -> 
-    (sel h' y = sel h y) /\ 
-    (sel h' x = sel h x + sel h y) /\ 
-    (sel h' hi = sel h hi))
-    (p1_r x y hi h))
+val p1_x (x y hi : id) (h:heap) :
+  Lemma (requires (x <> y /\ x <> hi /\ y <> hi))
+    (ensures (let h' = p1_r x y hi h in
+      (sel h' y = sel h y) /\
+      (sel h' x = sel h x + sel h y) /\
+      (sel h' hi = sel h hi)))
 let p1_x x y hi h = ()
 
-val ni_p1 (x y hi : id) (env:env) (h :rel heap) : 
-  Lemma 
+val ni_p1 (x y hi : id) (env:env) (h :rel heap) :
+  Lemma
   (requires (x <> y /\ x <> hi /\ y <> hi /\
             Low? (env x) /\
             Low? (env y) /\
             High? (env hi) /\
             low_equiv env h))
   (ensures  (low_equiv env (R (p1_r x y hi (R?.l h)) (p1_r x y hi (R?.r h)))))
-let ni_p1 x y hi env h = ()
+let ni_p1 x y hi env h = p1_x x y hi (R?.l h) ; p1_x x y hi (R?.r h)
